typing: style and reorg

src/typing/core.lean
@@ -1,5 +1,4 @@
-import env
-import exp
+import env exp
 
 namespace tts ------------------------------------------------------------------
 variables {V : Type} [decidable_eq V] -- Type of variable names
@@ -7,23 +6,23 @@ variables {V : Type} [decidable_eq V] -- Type of variable names
 open occurs exp typ sch
 
 inductive typing : env V → exp V → typ V → Prop
-  | var : Π {Γ : env V} {x : tagged V} {s : sch V} {ts : list (typ V)}
-    , x :~ s ∈ Γ
-    → s.arity = ts.length
-    → (∀ (t : typ V), t ∈ ts → lc t)
-    → lc s
-    → typing Γ (var free x) (open_typs ts s)
-  | app : Π {Γ : env V} {ef ea : exp V} {t₁ t₂ : typ V}
-    , typing Γ ef (arr t₁ t₂)
-    → typing Γ ea t₁
-    → typing Γ (app ef ea) t₂
-  | lam : Π {v} {Γ : env V} {eb : exp V} {t₁ t₂ : typ V} (L : finset (tagged V))
-    , lc t₁
-    → (∀ {x : tagged V}, x ∉ L → typing (insert ⟨x, ⟨0, t₁⟩⟩ Γ) (open_var x eb) t₂)
-    → typing Γ (lam v eb) (arr t₁ t₂)
-  | let_ : Π {v} {Γ : env V} {ed eb : exp V} (sd : sch V) {tb : typ V} (Ld Lb : finset (tagged V))
-    , (∀ {xs : list (tagged V)}, xs.length = sd.arity → xs.nodup → (∀ x ∈ xs, x ∉ Ld) → typing Γ ed (open_vars xs sd))
-    → (∀ {x : tagged V}, x ∉ Lb → typing (insert ⟨x, sd⟩ Γ) (open_var x eb) tb)
-    → typing Γ (let_ v ed eb) tb
+| var : Π {Γ : env V} {x : tagged V} {s : sch V} {ts : list (typ V)},
+    x :~ s ∈ Γ →
+    s.arity = ts.length →
+    (∀ (t : typ V), t ∈ ts → lc t) →
+    lc s →
+    typing Γ (var free x) (open_typs ts s)
+| app : Π {Γ : env V} {ef ea : exp V} {t₁ t₂ : typ V},
+    typing Γ ef (arr t₁ t₂) →
+    typing Γ ea t₁ →
+    typing Γ (app ef ea) t₂
+| lam : Π {v} {Γ : env V} {eb : exp V} {t₁ t₂ : typ V} (L : finset (tagged V)),
+    lc t₁ →
+    (∀ {x : tagged V}, x ∉ L → typing (insert ⟨x, ⟨0, t₁⟩⟩ Γ) (open_var x eb) t₂) →
+    typing Γ (lam v eb) (arr t₁ t₂)
+| let_ : Π {v} {Γ : env V} {ed eb : exp V} (sd : sch V) {tb : typ V} (Ld Lb : finset (tagged V)),
+    (∀ {xs : list (tagged V)}, xs.length = sd.arity → xs.nodup → (∀ x ∈ xs, x ∉ Ld) → typing Γ ed (open_vars xs sd)) →
+    (∀ {x : tagged V}, x ∉ Lb → typing (insert ⟨x, sd⟩ Γ) (open_var x eb) tb) →
+    typing Γ (let_ v ed eb) tb
 
 end /- namespace -/ tts --------------------------------------------------------
