src/typing/props.lean
@@ -2,7 +2,7 @@ import .core
 
 namespace tts ------------------------------------------------------------------
 namespace typing ---------------------------------------------------------------
-variables {V : Type} -- Type of variable names
+variables {V : Type} [decidable_eq V] -- Type of variable names
 variables {x y : tagged V} -- Variables
 variables {e ex e₁ : exp V} -- Expressions
 variables {t : typ V} -- Types
@@ -10,189 +10,182 @@ variables {s s' : sch V} -- Type schemes
 variables {Γ Γ₁ Γ₂ Γ₃ : env V} -- Environments
 variables {L : finset (tagged V)} -- Variable sets
 
-variables [decidable_eq V]
-
 open finmap occurs exp typ sch
 
-theorem weaken_middle
-: typing (Γ₁ ∪ Γ₃) e t
-→ disjoint (dom Γ₁) (dom Γ₂)
-→ disjoint (dom Γ₂) (dom Γ₃)
-→ disjoint (dom Γ₁) (dom Γ₃)
-→ typing (Γ₁ ∪ Γ₂ ∪ Γ₃) e t :=
-  begin
-    generalize Γeq : Γ₁ ∪ Γ₃ = Γ₁₃,
-    intros T dj₁₂ dj₂₃ dj₁₃,
-    induction T generalizing Γ₁ Γ₃,
-    case typing.var : Γ x s ts b ln_eq lts ls {
-      induction Γeq,
-      exact var (mem_union_middle_left dj₁₃ dj₂₃ b) ln_eq lts ls,
-    },
-    case typing.app : Γ ef ea t₁ t₂ Tf Ta ihf iha {
-      exact app (ihf Γeq dj₁₂ dj₂₃ dj₁₃) (iha Γeq dj₁₂ dj₂₃ dj₁₃),
-    },
-    case typing.lam : v Γ eb t₁ t₂ L lt₁ Ft₂ ihb {
-      apply lam (L ∪ dom (Γ₁ ∪ Γ₂ ∪ Γ₃)) lt₁,
-      introv nm,
+theorem weaken_middle :
+  disjoint (dom Γ₁) (dom Γ₂) →
+  disjoint (dom Γ₂) (dom Γ₃) →
+  disjoint (dom Γ₁) (dom Γ₃) →
+  typing (Γ₁ ∪ Γ₃) e t →
+  typing (Γ₁ ∪ Γ₂ ∪ Γ₃) e t :=
+begin
+  generalize Γeq : Γ₁ ∪ Γ₃ = Γ₁₃,
+  intros dj₁₂ dj₂₃ dj₁₃ T,
+  induction T generalizing Γ₁ Γ₃,
+  case typing.var : Γ x s ts b ln_eq lts ls {
+    induction Γeq,
+    exact var (mem_union_middle_left dj₁₃ dj₂₃ b) ln_eq lts ls,
+  },
+  case typing.app : Γ ef ea t₁ t₂ Tf Ta ihf iha {
+    exact app (ihf Γeq dj₁₂ dj₂₃ dj₁₃) (iha Γeq dj₁₂ dj₂₃ dj₁₃),
+  },
+  case typing.lam : v Γ eb t₁ t₂ L lt₁ Ft₂ ihb {
+    apply lam (L ∪ dom (Γ₁ ∪ Γ₂ ∪ Γ₃)) lt₁,
+    introv nm,
+    simp [not_or_distrib, and_assoc] at nm,
+    rw [←insert_union, ←insert_union],
+    induction Γeq,
+    exact ihb nm.1 insert_union
+      (disjoint_keys_insert_left.mpr ⟨nm.2.1, dj₁₂⟩)
+      dj₂₃
+      (disjoint_keys_insert_left.mpr ⟨nm.2.2.2, dj₁₃⟩),
+  },
+  case typing.let_ : v Γ ed eb sd tb Ld Lb _ _ ihd ihb {
+    apply let_ sd (Ld ∪ dom (Γ₁ ∪ Γ₂ ∪ Γ₃)) (Lb ∪ dom (Γ₁ ∪ Γ₂ ∪ Γ₃)),
+    { introv ln_eq nd nm,
+      simp [not_or_distrib, and_assoc] at nm,
+      exact ihd ln_eq nd (λ _ h, (nm _ h).1) Γeq dj₁₂ dj₂₃ dj₁₃ },
+    { introv nm,
       simp [not_or_distrib, and_assoc] at nm,
       rw [←insert_union, ←insert_union],
       induction Γeq,
       exact ihb nm.1 insert_union
         (disjoint_keys_insert_left.mpr ⟨nm.2.1, dj₁₂⟩)
-        dj₂₃ 
-        (disjoint_keys_insert_left.mpr ⟨nm.2.2.2, dj₁₃⟩),
-    },
-    case typing.let_ : v Γ ed eb sd tb Ld Lb _ _ ihd ihb {
-      apply let_ sd (Ld ∪ dom (Γ₁ ∪ Γ₂ ∪ Γ₃)) (Lb ∪ dom (Γ₁ ∪ Γ₂ ∪ Γ₃)),
-      { introv ln_eq nd nm,
-        simp [not_or_distrib, and_assoc] at nm,
-        exact ihd ln_eq nd (λ _ h, (nm _ h).1) Γeq dj₁₂ dj₂₃ dj₁₃ },
-      { introv nm,
-        simp [not_or_distrib, and_assoc] at nm,
-        rw [←insert_union, ←insert_union],
-        induction Γeq,
-        apply ihb nm.1 insert_union
-          (disjoint_keys_insert_left.mpr ⟨nm.2.1, dj₁₂⟩)
-          dj₂₃ 
-          (disjoint_keys_insert_left.mpr ⟨nm.2.2.2, dj₁₃⟩) }
-    }
-  end
+        dj₂₃
+        (disjoint_keys_insert_left.mpr ⟨nm.2.2.2, dj₁₃⟩) }
+  }
+end
 
-theorem weaken
-: typing Γ₂ e t
-→ disjoint (dom Γ₁) (dom Γ₂)
-→ typing (Γ₁ ∪ Γ₂) e t :=
-  begin
-    intros T dj,
-    rw ←empty_union Γ₂ at T,
-    rw ←empty_union Γ₁ at ⊢,
-    exact weaken_middle T (finset.disjoint_empty_left _) dj (finset.disjoint_empty_left _)
-  end
+theorem weaken :
+  disjoint (dom Γ₁) (dom Γ₂) →
+  typing Γ₂ e t →
+  typing (Γ₁ ∪ Γ₂) e t :=
+begin
+  intros dj T,
+  rw ←empty_union Γ₂ at T,
+  rw ←empty_union Γ₁ at ⊢,
+  exact weaken_middle (finset.disjoint_empty_left _) dj (finset.disjoint_empty_left _) T
+end
 
 lemma ne_of_nm : x ∉ L ∪ dom (Γ₁ ∪ finmap.singleton (y :~ s) ∪ Γ₂) → y ≠ x :=
-  by simp [not_or_distrib]; tauto
+by simp [not_or_distrib]; tauto
 
 lemma nmL_of_nm : x ∉ L ∪ dom (Γ₁ ∪ finmap.singleton (y :~ s) ∪ Γ₂) → x ∉ L :=
-  by simp [not_or_distrib]; tauto
+by simp [not_or_distrib]; tauto
 
 lemma nmΓ₂_of_nm : x ∉ L ∪ dom (Γ₁ ∪ finmap.singleton (y :~ s) ∪ Γ₂) → x ∉ dom Γ₂ :=
-  by simp [not_or_distrib]; tauto
+by simp [not_or_distrib]; tauto
 
-lemma nm_ins : x ∉ dom (Γ₁ ∪ Γ₂) → y ∉ L ∪ dom (Γ₁ ∪ finmap.singleton (x :~ s) ∪ Γ₂)
-→ x ∉ dom (insert (binding.mk y s') Γ₁ ∪ Γ₂) :=
-  by simp [not_or_distrib]; tauto
+lemma nm_ins : x ∉ dom (Γ₁ ∪ Γ₂) → y ∉ L ∪ dom (Γ₁ ∪ finmap.singleton (x :~ s) ∪ Γ₂) →
+  x ∉ dom (insert (binding.mk y s') Γ₁ ∪ Γ₂) :=
+by simp [not_or_distrib]; tauto
 
-theorem subst_weaken
-: typing (Γ₁ ∪ finmap.singleton (x :~ s) ∪ Γ₂) e t
-→ disjoint (dom Γ₁) (dom Γ₂)
-→ x ∉ dom (Γ₁ ∪ Γ₂)
-→ (∀ {ts : list (typ V)}, s.arity = ts.length → (∀ (t : typ V), t ∈ ts → lc t) → typing Γ₂ ex (open_typs ts s))
-→ lc ex
-→ typing (Γ₁ ∪ Γ₂) (subst x ex e) t :=
-  begin
-    generalize Γeq : Γ₁ ∪ finmap.singleton (x :~ s) ∪ Γ₂ = Γ₁₂,
-    intros T dj nmd Tex lex,
-    induction T generalizing Γ₁ Γ₂ x s ex,
-    case typing.var : Γ y s' ts b ln_eq lts ls {
-      induction Γeq, 
-      have b : y :~ s' ∈ Γ₁ ∨ y :~ s' ∈ finmap.singleton (x :~ s) ∨ y :~ s' ∈ Γ₂ :=
-        (or_assoc _ _).mp (or.imp_left mem_of_mem_union (mem_of_mem_union b)),
-      by_cases h : x = y,
-      { induction h,
-        simp [not_or_distrib] at nmd,
-        rcases b with m | m | m,
-        { exact absurd (mem_keys_of_mem m) nmd.1 },
-        { simp at m, induction m, simp [weaken (Tex ln_eq lts) dj] },
-        { exact absurd (mem_keys_of_mem m) nmd.2 } },
-      { rcases b with m | m | m,
-        { simp [h, var ((mem_union dj).mpr (or.inl m)) ln_eq lts ls] },
-        { simp at m, exact absurd m.1.symm h },
-        { simp [h, var ((mem_union dj).mpr (or.inr m)) ln_eq lts ls] } }
-    },
-    case typing.app : Γ ef ea t₁ t₂ Tf Ta ihf iha {
-      exact app (ihf Γeq dj nmd @Tex lex) (iha Γeq dj nmd @Tex lex)
-    },
-    case typing.lam : v Γ eb t₁ t₂ L lt₁ Ft₂ ihb {
-      apply lam (L ∪ dom (Γ₁ ∪ finmap.singleton (x :~ s) ∪ Γ₂)) lt₁,
-      induction Γeq, 
+theorem subst_weaken :
+  disjoint (dom Γ₁) (dom Γ₂) →
+  x ∉ dom (Γ₁ ∪ Γ₂) →
+  lc ex →
+  (∀ {ts : list (typ V)}, s.arity = ts.length → (∀ (t : typ V), t ∈ ts → lc t) → typing Γ₂ ex (open_typs ts s)) →
+  typing (Γ₁ ∪ finmap.singleton (x :~ s) ∪ Γ₂) e t →
+  typing (Γ₁ ∪ Γ₂) (subst x ex e) t :=
+begin
+  generalize Γeq : Γ₁ ∪ finmap.singleton (x :~ s) ∪ Γ₂ = Γ₁₂,
+  intros dj nmd lex Tex T,
+  induction T generalizing Γ₁ Γ₂ x s ex,
+  case typing.var : Γ y s' ts b ln_eq lts ls {
+    induction Γeq,
+    have b : y :~ s' ∈ Γ₁ ∨ y :~ s' ∈ finmap.singleton (x :~ s) ∨ y :~ s' ∈ Γ₂ :=
+      (or_assoc _ _).mp (or.imp_left mem_of_mem_union (mem_of_mem_union b)),
+    by_cases h : x = y,
+    { induction h,
+      simp [not_or_distrib] at nmd,
+      rcases b with m | m | m,
+      { exact absurd (mem_keys_of_mem m) nmd.1 },
+      { simp at m, induction m, simp [weaken dj (Tex ln_eq lts)] },
+      { exact absurd (mem_keys_of_mem m) nmd.2 } },
+    { rcases b with m | m | m,
+      { simp [h, var ((mem_union dj).mpr (or.inl m)) ln_eq lts ls] },
+      { simp at m, exact absurd m.1.symm h },
+      { simp [h, var ((mem_union dj).mpr (or.inr m)) ln_eq lts ls] } } },
+  case typing.app : Γ ef ea t₁ t₂ Tf Ta ihf iha {
+    exact app (ihf Γeq dj nmd lex @Tex) (iha Γeq dj nmd lex @Tex) },
+  case typing.lam : v Γ eb t₁ t₂ L lt₁ Ft₂ ihb {
+    apply lam (L ∪ dom (Γ₁ ∪ finmap.singleton (x :~ s) ∪ Γ₂)) lt₁,
+    induction Γeq,
+    intros y nm,
+    rw ←subst_open_var lex (ne_of_nm nm),
+    rw ←insert_union,
+    exact ihb (nmL_of_nm nm)
+      (by rw [insert_union, insert_union])
+      (disjoint_keys_insert_left.mpr ⟨by exact nmΓ₂_of_nm nm, dj⟩)
+      (nm_ins nmd nm)
+      lex
+      @Tex },
+  case typing.let_ : v Γ ed eb sd tb Ld Lb _ _ ihd ihb {
+    dsimp at ihd ihb,
+    apply let_ sd
+      (Ld ∪ dom (Γ₁ ∪ finmap.singleton (x :~ s) ∪ Γ₂))
+      (Lb ∪ dom (Γ₁ ∪ finmap.singleton (x :~ s) ∪ Γ₂)),
+    { intros xs ln_eq nd nm,
+      exact ihd ln_eq nd (λ _ h, nmL_of_nm (nm _ h)) Γeq dj nmd lex @Tex },
+    { induction Γeq,
       intros y nm,
       rw ←subst_open_var lex (ne_of_nm nm),
       rw ←insert_union,
-      apply ihb (nmL_of_nm nm)
+      exact ihb (nmL_of_nm nm)
         (by rw [insert_union, insert_union])
         (disjoint_keys_insert_left.mpr ⟨by exact nmΓ₂_of_nm nm, dj⟩)
         (nm_ins nmd nm)
-        @Tex
         lex
-    },
-    case typing.let_ : v Γ ed eb sd tb Ld Lb _ _ ihd ihb {
-      dsimp at ihd ihb,
-      apply let_ sd
-        (Ld ∪ dom (Γ₁ ∪ finmap.singleton (x :~ s) ∪ Γ₂))
-        (Lb ∪ dom (Γ₁ ∪ finmap.singleton (x :~ s) ∪ Γ₂)),
-      { intros xs ln_eq nd nm, apply ihd ln_eq nd (λ _ h, nmL_of_nm (nm _ h)) Γeq dj nmd @Tex lex },
-      { induction Γeq, 
-        intros y nm, 
-        rw ←subst_open_var lex (ne_of_nm nm),
-        rw ←insert_union,
-        apply ihb (nmL_of_nm nm)
-          (by rw [insert_union, insert_union])
-          (disjoint_keys_insert_left.mpr ⟨by exact nmΓ₂_of_nm nm, dj⟩)
-          (nm_ins nmd nm)
-          @Tex
-          lex }
-    }
-  end
+        @Tex } }
+end
 
 -- Expression substitution preserves typing.
-theorem exp_subst_preservation
-: x ∉ dom Γ
-→ typing (finmap.singleton (x :~ s) ∪ Γ) e₁ t
-→ (∀ {ts : list (typ V)}, s.arity = ts.length → (∀ (t : typ V), t ∈ ts → lc t) → typing Γ ex (open_typs ts s))
-→ lc ex
-→ typing Γ (subst x ex e₁) t :=
-  begin
-    intros nm T Tex lex,
-    rw ←empty_union (finmap.singleton (x :~ s)) at T,
-    rw ←empty_union Γ,
-    exact subst_weaken T (finset.disjoint_empty_left _) (by simp [nm]) @Tex lex
-  end
+theorem exp_subst_preservation :
+  x ∉ dom Γ →
+  lc ex →
+  (∀ {ts : list (typ V)}, s.arity = ts.length → (∀ (t : typ V), t ∈ ts → lc t) → typing Γ ex (open_typs ts s)) →
+  typing (finmap.singleton (x :~ s) ∪ Γ) e₁ t →
+  typing Γ (subst x ex e₁) t :=
+begin
+  intros nm lex Tex T,
+  rw ←empty_union (finmap.singleton (x :~ s)) at T,
+  rw ←empty_union Γ,
+  exact subst_weaken (finset.disjoint_empty_left _) (by simp [nm]) lex @Tex T
+end
 
 -- Typing implies a locally-closed expression
 theorem lc_exp (T : typing Γ e t) : lc e :=
-  begin
-    induction T,
-    case typing.var { simp },
-    case typing.app { simp * },
-    case typing.lam { simp [exp.lc_body, *], tauto },
-    case typing.let_ : v _ ed _ _ _ _ _ _ _ ihd {
-      have : lc ed := ihd
-        ((fresh.tagged v).pgenl_length _ _)
-        ((fresh.tagged v).pgenl_nodup _ _)
-        (λ _, (fresh.tagged v).pgenl_not_mem),
-      simp [exp.lc_body, *],
-      tauto
-    }
-  end
+begin
+  induction T,
+  case typing.var { simp },
+  case typing.app { simp * },
+  case typing.lam { simp [exp.lc_body, *], tauto },
+  case typing.let_ : v _ ed _ _ _ _ _ _ _ ihd {
+    have : lc ed := ihd
+      ((fresh.tagged v).pgenl_length _ _)
+      ((fresh.tagged v).pgenl_nodup _ _)
+      (λ _, (fresh.tagged v).pgenl_not_mem),
+    simp [exp.lc_body, *],
+    tauto
+  }
+end
 
 -- Typing implies a locally-closed type
-theorem lc_typ (T : typing Γ e t) : t.lc :=
-  begin
-    induction T,
-    case typing.var : _ x _ _ _ ln_eq lts ls {
-      exact lc_open_typs x.val ls ln_eq lts
-    },
-    case typing.app : Γ ef ea t₁ t₂ Tf Ta ihf iha {
-      simp at ihf, cases ihf with _ lt₂, exact lt₂
-    },
-    case typing.lam : v _ _ _ _ L lt₁ _ ihb {
-      dsimp at ihb,
-      simp [lt₁, ihb ((fresh.tagged v).gen_not_mem L)]
-    },
-    case typing.let_ : v _ _ _ _ _ _ Lb _ _ _ ihb {
-      exact ihb ((fresh.tagged v).gen_not_mem Lb)
-    }
-  end
+theorem lc_typ (T : typing Γ e t) : lc t :=
+begin
+  induction T,
+  case typing.var : _ x _ _ _ ln_eq lts ls {
+    exact lc_open_typs x.val ls ln_eq lts },
+  case typing.app : Γ ef ea t₁ t₂ Tf Ta ihf iha {
+    simp at ihf,
+    cases ihf with _ lt₂,
+    exact lt₂ },
+  case typing.lam : v _ _ _ _ L lt₁ _ ihb {
+    dsimp at ihb,
+    simp [lt₁, ihb ((fresh.tagged v).gen_not_mem L)] },
+  case typing.let_ : v _ _ _ _ _ _ Lb _ _ _ ihb {
+    exact ihb ((fresh.tagged v).gen_not_mem Lb) }
+end
 
 end /- namespace -/ typing -----------------------------------------------------
 end /- namespace -/ tts --------------------------------------------------------
